\documentclass[11pt]{article}

\usepackage{amsmath}
\usepackage{amssymb}
\usepackage{graphicx}
\usepackage{IEEEtrantools}
\usepackage{chemformula}
\usepackage{bm}
\usepackage{float}
\usepackage{hyperref}
\DeclareMathOperator*{\argmax}{argmax} % thin space, limits underneath in displays
\usepackage{subfig}

\setlength{\oddsidemargin}{0in}  % set margins
\setlength{\evensidemargin}{0in} %
\setlength{\textwidth}{6.5in}    %
\setlength{\textheight}{9.0in}   %
\setlength{\topmargin}{-0.5in}   %
\parskip=5pt
\setlength{\parindent}{0pt}


\begin{document}

The HDG local system can be written as:
\begin{align} 
    \left( \begin{array}{ccc} M&C &E \\ B&D&F \\ K&G&H  \end{array} \right) 
    \left( \begin{array}{c} \delta q \\ \delta u \\ \delta \hat{u}  \end{array} \right) = 
    \left( \begin{array}{c} Rq \\ Ru  \\ R\hat{u}   \end{array} \right)
\end{align}

Assuming $Rq=0$, we have:
\begin{align} 
    \left( \begin{array}{ccc} M&C &E \\ B&D&F \\ K&G&H  \end{array} \right) 
    \left( \begin{array}{c} \delta q \\ \delta u \\ \delta \hat{u}  \end{array} \right) = 
    \left( \begin{array}{c} 0 \\ Ru  \\ R\hat{u}   \end{array} \right)
\end{align}

To eliminate $\delta q$, we take the first equation:
\begin{align}
    M \delta q - C \delta u  + E \delta\hat{u} = 0\\
    \delta q = M^{-1}(C \delta u  - E \delta\hat{u})
\end{align}

Substituting into the second equation:

\begin{align}
    B \delta q + D \delta u  + F \delta\hat{u} = Ru\\
    BM^{-1}(C \delta u  - E \delta\hat{u}) + D \delta u  + F \delta\hat{u} = Ru\\
    (BM^{-1}C +D)\delta u +(F-BM^{-1}E) \delta\hat{u} = Ru
\end{align}

Substituting into the third equation:
\begin{align}
    K \delta q + G \delta u  + H \delta\hat{u} = R\hat{u} \\
    KM^{-1}(C \delta u  - E \delta\hat{u})+ G \delta u  + H \delta\hat{u} = R\hat{u} \\
    (KM^{-1}C + G)\delta u + (H- KM^{-1}E)\delta\hat{u} = R\hat{u}
\end{align}

Forming the reduced system
\begin{align} 
    \left( \begin{array}{cc} \tilde{D^*} & \tilde{F^*} \\ \tilde{G^*}&\tilde{H^*}  \end{array} \right) 
    \left( \begin{array}{c} \delta u \\ \delta \hat{u}   \end{array} \right) = 
    \left( \begin{array}{c} Ru  \\ R\hat{u}   \end{array} \right)
\end{align}

Where
\begin{align}
    \tilde{D^*} = BM^{-1}C +D\\
    \tilde{F^*} = F-BM^{-1}E\\
    \tilde{G^*} = KM^{-1}C + G\\
    \tilde{H^*} = H- KM^{-1}E\\
\end{align}


\end{document}
